some struggle for refinement from impl to protocol (I need to reconstruct the codes, so commit)

ironfleet/src/Dafny/Distributed/Impl/Raft/QRelations.i.dfy
@@ -9,48 +9,106 @@ import opened Raft__Server_i
 import opened Raft__ServerScheduler_i
 
 
-predicate {:opaque} Q_RaftServer_Next_ProcessPacket(server:RaftServer, server':RaftServer, ios:seq<RaftIo>)
-{
-  RaftServerNextProcessPacket(server, server', ios)
-}
-
 predicate {:opaque} Q_RaftScheduler_Next(sched:RaftServerScheduler, sched':RaftServerScheduler, ios:seq<RaftIo>)
 {
   RaftServerSchedulerNext(sched, sched', ios)
 }
 
-predicate {:opaque} Q_RaftServer_NoReceive_Next(server:RaftServer, nextActionIndex:int, server':RaftServer, ios:seq<RaftIo>)
+predicate {:opaque} Q_RaftServer_Next_ProcessPacket(server:RaftServer, server':RaftServer, ios:seq<RaftIo>)
 {
-  RaftServerNoReceiveNext(server, nextActionIndex, server', ios)
+  RaftServerNextProcessPacket(server, server', ios)
 }
 
-lemma lemma_EstablishQLSchedulerNext(server:RaftServer, server':RaftServer, ios:seq<RaftIo>, sched:RaftServerScheduler, sched':RaftServerScheduler)
-  requires 0 <= sched.nextActionIndex < RaftServerNumActions()
-  requires sched.nextActionIndex == 0 ==> Q_RaftServer_Next_ProcessPacket(server, server', ios)
-  requires sched.nextActionIndex == 1 ==> Q_RaftServer_NoReceive_Next(server, sched.nextActionIndex, server', ios)
-  requires sched.server == server
-  requires sched'.server == server'
-  requires sched'.nextActionIndex == (sched.nextActionIndex+1)%RaftServerNumActions()
-  // TOPROVE
-  // ensures Q_RaftScheduler_Next(sched, sched', ios)
+predicate Q_RaftServer_Next_ReadClock_Leader(server:RaftServer, server':RaftServer, clock:int, sent_packets:seq<RaftPacket>)
 {
-  reveal Q_RaftServer_Next_ProcessPacket();
-  reveal Q_RaftServer_NoReceive_Next();
-  reveal Q_RaftScheduler_Next();
+  RaftServerNextReadClock_Leader(server, server', clock, sent_packets)
 }
 
-lemma lemma_EstablishQRaftServerNextProcessPacketFromTimeout(server:RaftServer, server':RaftServer, ios:seq<RaftIo>)
-  requires |ios|==1
-  requires ios[0].LIoOpTimeoutReceive?
-  requires server==server'
-  ensures Q_RaftServer_Next_ProcessPacket(server, server', ios)
+predicate Q_RaftServer_Next_ReadClock_NonLeader(server:RaftServer, server':RaftServer, clock:int, sent_packets:seq<RaftPacket>)
 {
-  reveal Q_RaftServer_Next_ProcessPacket();
+  RaftServerNextReadClock_NonLeader(server, server', clock, sent_packets)
 }
 
-predicate {:opaque} Q_RaftServerScheduler_Next(s:RaftServerScheduler, s':RaftServerScheduler, ios:seq<RaftIo>)
+predicate {:opaque} Q_RaftServer_Next_ReadClock(server:RaftServer, server':RaftServer, ios:seq<RaftIo>)
 {
-  RaftServerSchedulerNext(s, s', ios)
+  RaftServerNextReadClock(server, server', ios)
+}
+
+predicate {:opaque} Q_RaftServer_Next_CommitAndApply(server:RaftServer, server':RaftServer, ios:seq<RaftIo>)
+{
+  RaftServerNextCommitAndApply(server, server', ios)
+}
+
+// predicate {:opaque} Q_RaftServer_Next_Process_AppendEntries(server:RaftServer, server':RaftServer, raft_packet:RaftPacket, clock:int, sent_packets:seq<RaftPacket>)
+// {
+//   // raft_packet.msg.RaftMessage_AppendEntries? && RaftServerNextProcessAppendEntries(server, server', raft_packet, clock, sent_packets)
+//   true
+// }
+
+// predicate Establish_Q_RaftServer_Next_ProcessPacket_preconditions(server:RaftServer, server':RaftServer, raft_packet:RaftPacket, clock:int, sent_packets:seq<RaftPacket>, ios:seq<RaftIo>)
+// {
+//   && sent_packets == ExtractSentPacketsFromIos(ios)
+//   && clock == SpontaneousClock(ios)
+//   // && raft_packet.msg.RaftMessage_AppendEntries?
+//   // && Q_RaftServer_Next_Process_AppendEntries(server, server', raft_packet, clock, sent_packets)
+//   && (
+//     || (raft_packet.msg.RaftMessage_Invalid? && (server == server' && sent_packets == []))
+//     || (raft_packet.msg.RaftMessage_AppendEntries? && Q_RaftServer_Next_Process_AppendEntries(server, server', raft_packet, clock, sent_packets))
+//     // || (raft_packet.msg.RaftMessage_RequestVote? && (server == server' && sent_packets == []))
+//     || (raft_packet.msg.RaftMessage_AppendEntriesReply? && (server == server' && sent_packets == []))
+//     || (raft_packet.msg.RaftMessage_RequestVote? && (server == server' && sent_packets == []))
+//     || (raft_packet.msg.RaftMessage_RequestVoteReply? && (server == server' && sent_packets == []))
+//     || (raft_packet.msg.RaftMessage_Request? && (server == server' && sent_packets == []))
+//     || (raft_packet.msg.RaftMessage_Reply? && (server == server' && sent_packets == []))
+//   )
+// }
+
+// lemma lemma_EstablishQLReplicaNextProcessPacket(server:RaftServer, server':RaftServer, raft_packet:RaftPacket, clock:int, sent_packets:seq<RaftPacket>, ios:seq<RaftIo>)
+//   requires |ios| >= 1
+//   requires ios[0].LIoOpReceive?
+//   requires |ios| >= 2 ==> (
+//     || (ios[1].LIoOpReadClock? && AllIosAreSends(ios[2..]))
+//     || (ios[1].LIoOpSend? && AllIosAreSends(ios[1..]))
+//   )
+//   requires sent_packets == ExtractSentPacketsFromIos(ios)
+//   requires Establish_Q_RaftServer_Next_ProcessPacket_preconditions(server, server', raft_packet, clock, sent_packets, ios)
+//   ensures Q_RaftServer_Next_ProcessPacket(server, server', ios)
+// {
+//   reveal Q_RaftServer_Next_Process_AppendEntries();
+
+//   reveal Q_RaftServer_Next_ProcessPacket();
+// }
+
+// lemma lemma_EstablishQRaftServerSchedulerNext(server:RaftServer, server':RaftServer, ios:seq<RaftIo>, sched:RaftServerScheduler, sched':RaftServerScheduler)
+//   requires 0 <= sched.nextActionIndex <= RaftServerNumActions() - 1
+//   requires sched.nextActionIndex == 0 ==> Q_RaftServer_Next_ProcessPacket(server, server', ios)
+//   requires sched.nextActionIndex == 1 ==> Q_RaftServer_Next_ReadClock(server, server', ios)
+//   requires sched.nextActionIndex == 2 ==> Q_RaftServer_Next_CommitAndApply(server, server', ios)
+//   requires sched.server == server
+//   requires sched'.server == server'
+//   requires sched'.nextActionIndex == (sched.nextActionIndex+1) % RaftServerNumActions()
+//   // TOPROVE
+//   ensures Q_RaftScheduler_Next(sched, sched', ios)
+// {
+//   reveal Q_RaftServer_Next_ProcessPacket();
+//   reveal Q_RaftServer_Next_ReadClock();
+//   reveal Q_RaftScheduler_Next();
+//   assert sched'.nextActionIndex == (sched.nextActionIndex + 1) % RaftServerNumActions();
+//   assert Q_RaftScheduler_Next(sched, sched', ios);
+// }
+
+// lemma lemma_EstablishQRaftServerNextProcessPacketFromTimeout(server:RaftServer, server':RaftServer, ios:seq<RaftIo>)
+//   requires |ios|==1
+//   requires ios[0].LIoOpTimeoutReceive?
+//   requires server==server'
+//   ensures Q_RaftServer_Next_ProcessPacket(server, server', ios)
+// {
+//   reveal Q_RaftServer_Next_ProcessPacket();
+// }
+
+predicate {:opaque} Q_RaftServerScheduler_Next(server:RaftServerScheduler, server':RaftServerScheduler, ios:seq<RaftIo>)
+{
+  RaftServerSchedulerNext(server, server', ios)
 }
 
 predicate AllIosAreSends(ios:seq<RaftIo>)
