ironfleet/src/Dafny/Distributed/Impl/Raft/ServerImplNoReceiveClock.i.dfy
@@ -13,6 +13,8 @@ include "QRelations.i.dfy"
 include "ServerImpl.i.dfy"
 include "ServerImplDelivery.i.dfy"
 // include "NetRSL.i.dfy"
+// DEBUG
+include "../../Protocol/Common/UpperBound.s.dfy"
 
 module Raft__ServerImplNoReceiveClock_i {
 
@@ -33,12 +35,13 @@ import opened Raft__QRelations_i
 import opened Raft__ServerImpl_i
 import opened Raft__ServerImplDelivery_i
 import opened Raft__Types_i
+import opened Common__UpperBound_s
 
 method Server_Next_NoReceive_ReadClock(server_impl:ServerImpl)
   returns (ok:bool, ghost net_event_log:seq<NetEvent>, ghost ios:seq<RaftIo>)
   requires server_impl.nextActionIndex == 1
   requires server_impl.Valid()
-  modifies server_impl.repr, server_impl.random_generator
+  modifies server_impl, server_impl.repr, server_impl.random_generator
   ensures server_impl.repr == old(server_impl.repr)
   ensures server_impl.net_client != null
   ensures ok == NetClientOk(server_impl.net_client)
@@ -48,7 +51,7 @@ method Server_Next_NoReceive_ReadClock(server_impl:ServerImpl)
             && server_impl.Env() == old(server_impl.Env())
             && server_impl.nextActionIndex == old(server_impl.nextActionIndex)
             // TOPROVE
-            // && Q_RaftServer_NoReceive_Next(old(server_impl.AbstractifyToRaftServer()), server_impl.nextActionIndex as int, server_impl.AbstractifyToRaftServer(), ios)
+            // && Q_RaftServer_Next_ReadClock(old(server_impl.AbstractifyToRaftServer()), server_impl.AbstractifyToRaftServer(), ios)
             && OnlySentMarshallableData(net_event_log)
             && RawIoConsistentWithSpecIO(net_event_log, ios)
             && old(server_impl.Env().net.history()) + net_event_log == server_impl.Env().net.history()
@@ -59,91 +62,97 @@ method Server_Next_NoReceive_ReadClock(server_impl:ServerImpl)
   net_event_log := [];
   ios := [];
 
-  if server_impl.nextActionIndex == 1 {
-    var clock,clock_event := ReadClock(server_impl.net_client);
-    ghost var clock_io := LIoOpReadClock(clock.t as int);
-    ghost var ios_head := [clock_io];
-    ghost var log_head := [clock_event];
-    ghost var log_tail := [];
-    ghost var ios_tail := [];
-    net_event_log := log_head;
-    ios := ios_head;
-    ghost var preDeliveryHistory := server_impl.Env().net.history();
-    // Default return
-    net_event_log := log_head;
-    ios := ios_head;
-    ok := true;
+  var clock,clock_event := ReadClock(server_impl.net_client);
+  ghost var clock_io := LIoOpReadClock(clock.t as int);
+  ghost var ios_head := [clock_io];
+  ghost var log_head := [clock_event];
+  ghost var log_tail := [];
+  ghost var ios_tail := [];
+  net_event_log := log_head;
+  ios := ios_head;
+  ghost var preDeliveryHistory := server_impl.Env().net.history();
+  // Default return
+  net_event_log := log_head;
+  ios := ios_head;
+  ok := true;
 
-    if (server_impl.role.Leader?) {
-      if (clock.t >= server_impl.next_heartbeat_time) {
-        var const_params := server_impl.config.global_config.params;
-        var next_heartbeat_time := UpperBoundedAdditionImpl(clock.t, const_params.heartbeat_timeout, const_params.max_integer_value);
-        server_impl.next_heartbeat_time := next_heartbeat_time;
-        
-        // Create packets
-        var outbound_packets:seq<CPacket> := [];
-        ok, outbound_packets := Server_CreateAppendEntriesForAll(server_impl, true);
-        if (!ok) {
-          print "prepare AppendEntries failed\n";
-          ok := true;
-          return;
-        }
-        assert |outbound_packets| <= |server_impl.config.global_config.server_eps| <= 0xFFFF_FFFF_FFFF_FFFF;
-        assert (forall p :: p in outbound_packets ==> CPacketIsSendable(p));
-        ok, log_tail, ios_tail := DeliverOutboundPackets(server_impl, PacketSequence(outbound_packets));
-        if (!ok) { return; }
-        ios := ios_head + ios_tail;
-        net_event_log := log_head + log_tail;
-        // print "I broadcast heartbeat!\n";
-        assert forall i::0<=i<|log_tail| ==> AbstractifyNetEventToRaftIo(log_tail[i]) == ios_tail[i];
-        assert forall i::0<=i<|log_tail| ==> log_tail[i].LIoOpSend? && ios_tail[i].LIoOpSend?;
-        assert forall i :: 1 <= i < |net_event_log| ==> net_event_log[i].LIoOpSend?;
-        assert forall i :: 0 <= i < |net_event_log| - 1 ==> net_event_log[i].LIoOpReceive? || net_event_log[i+1].LIoOpSend?;
-      } else {
-        net_event_log := log_head;
-        ios := ios_head;
-      }
+  if (server_impl.role.Leader?) {
+    if (clock.t >= server_impl.next_heartbeat_time) {
+      var const_params := server_impl.config.global_config.params;
+      // Create heartbeat packets
+      var outbound_packets:seq<CPacket> := [];
+      outbound_packets := Server_CreateAppendEntriesForAll(server_impl, true);
+      assert |outbound_packets| <= |server_impl.config.global_config.server_eps| <= 0xFFFF_FFFF_FFFF_FFFF;
+      assert (forall p :: p in outbound_packets ==> CPacketIsSendable(p));
+      ok, log_tail, ios_tail := DeliverOutboundPackets(server_impl, PacketSequence(outbound_packets));
+      if (!ok) { return; }
+      ios := ios_head + ios_tail;
+      net_event_log := log_head + log_tail;
+      // print "I broadcast heartbeat!\n";
+      assert forall i::0<=i<|log_tail| ==> AbstractifyNetEventToRaftIo(log_tail[i]) == ios_tail[i];
+      assert forall i::0<=i<|log_tail| ==> log_tail[i].LIoOpSend? && ios_tail[i].LIoOpSend?;
+      assert forall i :: 1 <= i < |net_event_log| ==> net_event_log[i].LIoOpSend?;
+      assert forall i :: 0 <= i < |net_event_log| - 1 ==> net_event_log[i].LIoOpReceive? || net_event_log[i+1].LIoOpSend?;
+
+      // Update fields of server_impl after delivering packets
+      var next_heartbeat_time := UpperBoundedAdditionImpl(clock.t, const_params.heartbeat_timeout, const_params.max_integer_value);
+      server_impl.next_heartbeat_time := next_heartbeat_time;
+      var raft_server := old(server_impl.AbstractifyToRaftServer());
+      var raft_server' := server_impl.AbstractifyToRaftServer();
+      assert Q_RaftServer_Next_ReadClock_Leader(raft_server, raft_server', clock.t as int, AbstractifyOutboundCPacketsToSeqOfRaftPackets(PacketSequence(outbound_packets)));
     } else {
-      if (clock.t >= server_impl.next_election_time) {
-        var const_params := server_impl.config.global_config.params;
-        var next_election_delta := server_impl.random_generator.NextInt(
-          const_params.min_election_timeout,
-          const_params.max_election_timeout
-        );
-        var next_election_time := UpperBoundedAdditionImpl(clock.t, next_election_delta, const_params.max_integer_value);
-        server_impl.next_election_time := next_election_time;
-        if (!ok) { return; }
-        print "My election timeout!!\n";
-        ios := [clock_io];
-        net_event_log := [clock_event];
-        // TODO: need to increase my term
-        if server_impl.current_term > 0xFFFF_FFFF_FFFF_FFFF - 1 {
-          ok := true;
-          return;
-        }
-        server_impl.current_term := server_impl.current_term + 1;
-        server_impl.BecomeCandidate();
-        var outbound_packets;
-        ok, outbound_packets := Server_CreateRequestVoteForAll(server_impl);
-        if (!ok) {
-          ok := true;
-          return;
-        }
-        assert |outbound_packets| <= |server_impl.config.global_config.server_eps| <= 0xFFFF_FFFF_FFFF_FFFF;
-        assert (forall p :: p in outbound_packets ==> CPacketIsSendable(p));
-        ok, log_tail, ios_tail := DeliverOutboundPackets(server_impl, PacketSequence(outbound_packets));
-        if (!ok) { return; }
-        ios := ios_head + ios_tail;
-        net_event_log := log_head + log_tail;
-        assert net_event_log[0].LIoOpReadClock?;
-        assert forall i::0<=i<|log_tail| ==> AbstractifyNetEventToRaftIo(log_tail[i]) == ios_tail[i];
-        assert forall i::0<=i<|log_tail| ==> log_tail[i].LIoOpSend? && ios_tail[i].LIoOpSend?;
-        assert forall i :: 1 <= i < |net_event_log| ==> net_event_log[i].LIoOpSend?;
-        assert forall i :: 0 <= i < |net_event_log| - 1 ==> net_event_log[i].LIoOpReceive? || net_event_log[i+1].LIoOpSend?;
-      } else {
-        net_event_log := log_head;
-        ios := ios_head;
+      net_event_log := log_head;
+      ios := ios_head;
+    }
+  } else {
+    if (clock.t >= server_impl.next_election_time) {
+      var const_params := server_impl.config.global_config.params;
+      var next_election_delta := server_impl.random_generator.NextInt(
+        const_params.min_election_timeout,
+        const_params.max_election_timeout
+      );
+      print "My election timeout!!\n";
+      ios := [clock_io];
+      net_event_log := [clock_event];
+      // TODO: need to increase my term
+      if server_impl.current_term > 0xFFFF_FFFF_FFFF_FFFF - 1 {
+        ok := true;
+        return;
       }
+      server_impl.current_term := server_impl.current_term + 1;
+      server_impl.BecomeCandidate();
+      var outbound_packets;
+      ok, outbound_packets := Server_CreateRequestVoteForAll(server_impl);
+      if (!ok) {
+        ok := true;
+        return;
+      }
+      assert |outbound_packets| <= |server_impl.config.global_config.server_eps| <= 0xFFFF_FFFF_FFFF_FFFF;
+      assert (forall p :: p in outbound_packets ==> CPacketIsSendable(p));
+
+      var server_impl_before_deliver := server_impl;
+      ok, log_tail, ios_tail := DeliverOutboundPackets(server_impl, PacketSequence(outbound_packets));
+      if (!ok) { return; }
+      ios := ios_head + ios_tail;
+      net_event_log := log_head + log_tail;
+      assert net_event_log[0].LIoOpReadClock?;
+      assert forall i::0<=i<|log_tail| ==> AbstractifyNetEventToRaftIo(log_tail[i]) == ios_tail[i];
+      assert forall i::0<=i<|log_tail| ==> log_tail[i].LIoOpSend? && ios_tail[i].LIoOpSend?;
+      assert forall i :: 1 <= i < |net_event_log| ==> net_event_log[i].LIoOpSend?;
+      assert forall i :: 0 <= i < |net_event_log| - 1 ==> net_event_log[i].LIoOpReceive? || net_event_log[i+1].LIoOpSend?;
+
+      server_impl := server_impl_before_deliver;
+
+      // Update fields of server_impl after delivering packets
+      var next_election_time := UpperBoundedAdditionImpl(clock.t, next_election_delta, const_params.max_integer_value);
+      server_impl.next_election_time := next_election_time;
+
+      var raft_server := old(server_impl.AbstractifyToRaftServer());
+      var raft_server' := server_impl.AbstractifyToRaftServer();
+      // assert RaftServerNextReadClock_NonLeader(raft_server, raft_server', clock.t as int, AbstractifyOutboundCPacketsToSeqOfRaftPackets(PacketSequence(outbound_packets)));
+    } else {
+      net_event_log := log_head;
+      ios := ios_head;
     }
   }
 }
